first synthesis of freeze code

src/Specific/ArithmeticSynthesisTest.v
@@ -20,6 +20,7 @@ Section Ops51.
   (* These definitions will need to be passed as Ltac arguments (or
   cleverly inferred) when things are eventually automated *)
   Definition sz := 5%nat.
+  Definition bitwidth := 64.
   Definition s : Z := 2^255.
   Definition c : list B.limb := [(1, 19)].
   Definition coef_div_modulus : nat := 2. (* add 2*modulus before subtracting *)
@@ -33,15 +34,14 @@ Section Ops51.
                      let si := Z.log2 s * i in
                      2 ^ ((si/sz) + (if dec ((si/sz)*sz=si) then 0 else 1)).
   Definition sz2 := Eval vm_compute in ((sz * 2) - 1)%nat.
+  Definition m_enc :=
+    Eval vm_compute in (Positional.encode (modulo:=modulo) (div:=div) (n:=sz) wt (s-Associational.eval c)).
   Definition coef := (* subtraction coefficient *)
     Eval vm_compute in
-      ( let p := Positional.encode
-                   (modulo:=modulo) (div:=div) (n:=sz)
-                   wt (s-Associational.eval c) in
-        (fix addp (acc: Z^sz) (ctr : nat) : Z^sz :=
+      ((fix addm (acc: Z^sz) (ctr : nat) : Z^sz :=
          match ctr with
          | O => acc
-         | S n => addp (Positional.add_cps wt acc p id) n
+         | S n => addm (Positional.add_cps wt acc m_enc id) n
         end) (Positional.zeros sz) coef_div_modulus).
   Definition coef_mod : mod_eq m (Positional.eval (n:=sz) wt coef) 0 := eq_refl.
 
@@ -187,6 +187,83 @@ Section Ops51.
     solve_op_F wt x. reflexivity.
   Defined.
 
+  Require Import Crypto.Arithmetic.Saturated.
+
+  Section PreFreeze.
+    Definition add_get_carry (s x y : Z) : Z * Z :=
+        dlet z := (x + y)%RT in (Core.modulo z s, Core.div z s).
+
+    Lemma add_get_carry_mod s x y :
+        fst (add_get_carry s x y) = (x + y) mod s.
+    Proof.
+        cbv [add_get_carry]; autorewrite with cancel_pair.
+        apply modulo_correct.
+    Qed.
+
+    Lemma add_get_carry_div s x y :
+        snd (add_get_carry s x y) = (x + y) / s.
+    Proof.
+        cbv [add_get_carry]; autorewrite with cancel_pair.
+        apply div_correct.
+    Qed.
+
+    Lemma wt_pos i : wt i > 0.
+    Proof.
+        apply Z.lt_gt.
+        apply Z.pow_pos_nonneg; zero_bounds; try break_match; vm_decide.
+    Qed.
+
+    Lemma wt_multiples i : wt (S i) mod (wt i) = 0.
+    Admitted.
+
+    Lemma wt_divides_full_pos i : wt (S i) / wt i > 0.
+    Proof.
+        pose proof (wt_divides_full i).
+        apply Z.div_positive_gt_0; auto using wt_pos.
+        apply wt_multiples.
+    Qed.
+
+    Context {select_cps : forall n, Z -> Z^n -> forall {T}, (Z^n->T) -> T}
+            {select : forall n, Z -> Z^n -> Z^n}
+            {select_id : forall n cond x T f, @select_cps n cond x T f = f (select n cond x)}
+            {eval_select : forall n cond x,
+                B.Positional.eval wt (select n cond x) = if dec (cond = 0) then 0 else B.Positional.eval wt x}
+    .
+
+    Hint Rewrite select_id : uncps.
+    Hint Rewrite eval_select : push_basesystem_eval.
+
+    Hint Opaque freeze : uncps.
+    Hint Rewrite freeze_id : uncps.
+  End PreFreeze.
+  
+  Definition freeze_sig :
+    {freeze : (Z^sz -> Z^sz)%type |
+     forall a : Z^sz,
+         (0 <= Positional.eval wt a < 2 * Z.pos m)->
+                 let eval := Positional.Fdecode (m := m) wt in
+                 eval (freeze a) = eval a}.
+  Proof.
+    eexists; cbv beta zeta; intros.
+    pose proof wt_nonzero. pose proof wt_pos.
+    pose proof div_mod. pose proof wt_divides_full_pos.
+    pose proof wt_multiples.
+    pose proof add_get_carry_mod.
+    pose proof add_get_carry_div.
+    pose proof div_correct. pose proof modulo_correct.
+    pose proof select_id. pose proof eval_select.
+    let x := constr:(freeze (n:=5) (add_get_carry:=add_get_carry) (div:=div) (modulo:=modulo) (select_cps:=select_cps) wt m_enc a) in
+    F_mod_eq;
+      transitivity (Positional.eval wt x); repeat autounfold;
+        [ | autorewrite with uncps push_id push_basesystem_eval;
+            rewrite eval_freeze with (c:=c);
+            try eassumption; try omega; try reflexivity; vm_decide].
+   cbv[mod_eq]; apply f_equal2;
+     [  | reflexivity ]; apply f_equal.
+   cbv - [runtime_opp runtime_add runtime_mul runtime_shr runtime_and Let_In add_get_carry].
+   reflexivity.
+  Defined.
+  
   Definition ring_51 :=
     (Ring.ring_by_isomorphism
          (F := F m)
